Test/civl/regression-tests/linear_types.bpl
@@ -7,13 +7,6 @@ atomic action {:layer 1, 2} A3({:linear_in} path: Lset int, {:linear_out} l: Lse
     call Lset_Split(path', l);
 }
 
-atomic action {:layer 1, 2} A4({:linear_in} path: Lset int, l: Lval int) returns (path': Lset int) {
-    call path' := Lset_Empty();
-    call Lset_Put(path', path);
-    call Lval_Put(path', l);
-    call Lval_Split(path', l);
-}
-
 atomic action {:layer 1, 2} A5({:linear_in} path: Lheap int) returns (path': Lheap int) {
     path' := path;
 }
@@ -22,22 +15,9 @@ var {:layer 0, 2} g: Lheap int;
 
 datatype Foo { Foo(f: Lheap int) }
 
-atomic action {:layer 1, 2} A8({:linear_out} l: Lval int, {:linear_in} path: Lset int) returns (path': Lset int)
-{
-    path' := path;
-    call Lval_Split(path', l);
-}
-
 atomic action {:layer 1, 2} A10({:linear_in} a: Foo) returns (b: Foo)
 {
     var x: Lheap int;
     Foo(x) := a;
     b := Foo(x);
-}
-
-datatype Bar { Bar(x: Lval int, y: int) }
-
-atomic action {:layer 1, 2} A11({:linear_in} a: Lval int) returns (b: Bar)
-{
-    b := Bar(a, 3+4);
 }
